Prove convert_formula_to_rformula.

formulae.v
@@ -4,6 +4,12 @@ Require Import Utf8 List.
 From larith Require Import tactics notations utilities.
 Import ListNotations.
 
+(*
+A note on variable indices: To greatly simplify certain proofs, we do not use
+absolute variable indices. Instead the existential quantifier pushes a value on
+the context stack, and a variable index refers to an index on the stack. It is
+always possible to translate absolute indices to these relative indices.
+*)
 Section First_order_formulae.
 
 Variable atom : Type.
@@ -13,81 +19,225 @@ Inductive wff :=
   | WffAtom (a : atom)
   | WffAnd (φ ϕ : wff)
   | WffNot (φ : wff)
-  | WffEx (i : nat) (φ : wff).
+  | WffEx (φ : wff).
 
 Variable domain : Type.
-Variable Holds : (nat -> domain) -> atom -> Prop.
+Variable Model : list domain -> atom -> Prop.
 
-(* Standard formula interpretation. *)
-Fixpoint Models (Γ : nat -> domain) (f : wff) :=
+Fixpoint Realizes (Γ : list domain) (f : wff) :=
   match f with
-  | WffAtom a   => Holds Γ a
-  | WffAnd φ ϕ  => Models Γ φ /\ Models Γ ϕ
-  | WffNot φ    => ¬Models Γ φ
-  | WffEx i φ   => ∃x, Models (Γ;;i↦x) φ
+  | WffAtom a  => Model Γ a
+  | WffAnd φ ϕ => Realizes Γ φ /\ Realizes Γ ϕ
+  | WffNot φ   => ¬Realizes Γ φ
+  | WffEx φ    => ∃x, Realizes (x :: Γ) φ
   end.
 
 End First_order_formulae.
 
-Arguments Models {_ _}.
-Notation "𝔄 |= ( φ )[ Γ ]" := (Models 𝔄 Γ φ)
-  (at level 20, format "𝔄  |=  ( φ )[ Γ ]").
+Arguments WffAtom {_}.
+Arguments WffAnd {_}.
+Arguments WffNot {_}.
+Arguments WffEx {_}.
+Arguments Realizes {_ _}.
 
-(* Atomic formulae for different languages. *)
-Section Languages.
+Notation model atom domain := (list domain -> atom -> Prop).
+Notation "¬` φ" := (WffNot φ) (at level 30, right associativity, format "¬` φ").
+Notation "φ ∧` ϕ" := (WffAnd φ ϕ) (right associativity, at level 35).
+Notation "∃[ φ ]" := (WffEx φ) (format "∃[ φ ]").
+Notation "A |= ( φ )[ Γ ]" := (Realizes A Γ φ)
+  (at level 20, format "A  |=  ( φ )[ Γ ]").
+
+Section Lemmas_about_realization.
+
+Variable dom atomA atomB : Type.
+Variable A : model atomA dom.
+Variable B : model atomB dom.
+
+Theorem realizes_ex φ ϕ :
+  (∀Γ, A |= (φ)[Γ] <-> B |= (ϕ)[Γ]) ->
+  ∀Γ, A |= (∃[φ])[Γ] <-> B |= (∃[ϕ])[Γ].
+Proof.
+intros eqv; simpl; split; intros [x Hx];
+exists x; apply eqv, Hx.
+Qed.
+
+Theorem realizes_and φ1 φ2 ϕ1 ϕ2 :
+  (∀Γ, A |= (φ1)[Γ] <-> B |= (ϕ1)[Γ]) ->
+  (∀Γ, A |= (φ2)[Γ] <-> B |= (ϕ2)[Γ]) ->
+  ∀Γ, A |= (φ1 ∧` φ2)[Γ] <-> B |= (ϕ1 ∧` ϕ2)[Γ].
+Proof.
+intros eqv1 eqv2; simpl; split; intros H.
+all: split; [apply eqv1|apply eqv2]; apply H.
+Qed.
+
+End Lemmas_about_realization.
+
+(* Atomic formulae for languages that we will be using. *)
+Section Atomic_formulae_for_linear_integer_arithmetic.
 
 Inductive std_term :=
   | Zero
-  | Succ (x : std_term)
-  | Add (x y : std_term)
-  | Var (i : nat).
+  | One
+  | Var (i : nat)
+  | Add (x y : std_term).
 
 Inductive std_atom :=
   | Std_eq (x y : std_term)
   | Std_le (x y : std_term).
 
 Inductive r_atom :=
-  | R_eq (i j : nat)
-  | R_le (i j : nat)
+  | R_zero (i : nat)
+  | R_one (i : nat)
   | R_add (i j k : nat)
-  | R_const (i n : nat).
+  | R_eq (i j : nat)
+  | R_le (i j : nat).
 
-End Languages.
+End Atomic_formulae_for_linear_integer_arithmetic.
 
 Notation formula := (wff std_atom).
 Notation rformula := (wff r_atom).
 
-Section Standard_models.
+Definition formula_atom := @WffAtom std_atom.
+Definition rformula_atom := @WffAtom r_atom.
 
-Fixpoint eval (Γ : nat -> nat) (x : std_term) :=
+Coercion formula_atom : std_atom >-> formula.
+Coercion rformula_atom : r_atom >-> rformula.
+
+(* Standard models of linear integer arithmetic. *)
+Section Standard_models_of_linear_integer_arithmetic.
+
+Fixpoint eval (Γ : list nat) (x : std_term) :=
   match x with
-  | Zero => 0
-  | Succ y => S (eval Γ y)
+  | Zero    => 0
+  | One     => 1
+  | Var i   => nth i Γ 0
   | Add x y => eval Γ x + eval Γ y
-  | Var i => Γ i
   end.
 
-Definition 𝔑 (Γ : nat -> nat) (a : std_atom) :=
+Definition Nat (Γ : list nat) (a : std_atom) :=
   match a with
   | Std_eq x y => eval Γ x = eval Γ y
-  | Std_le x y => eval Γ x <= eval Γ y
+  | Std_le x y => eval Γ x ≤ eval Γ y
   end.
 
-Definition 𝔑r (Γ : nat -> nat) (a : r_atom) :=
+Definition NatR (Γ : list nat) (a : r_atom) :=
+  let f := λ i, nth i Γ 0 in
   match a with
-  | R_eq i j => Γ i = Γ j
-  | R_le i j => Γ i <= Γ j
-  | R_add i j k => Γ i + Γ j = Γ k
-  | R_const i n => Γ i = n
+  | R_zero i    => f i = 0
+  | R_one i     => f i = 1
+  | R_add i j k => f i = f j + f k
+  | R_eq i j    => f i = f j
+  | R_le i j    => f i ≤ f j
   end.
 
-End Standard_models.
+End Standard_models_of_linear_integer_arithmetic.
 
-Section Embeddings.
+(* Embedding formula in rformula. *)
+Section Embedding_of_formula_in_rformula.
 
-Theorem convert_rformula_to_formula φ :
-  Σ ϕ, ∀Γ, 𝔑r |= (φ)[Γ] <-> 𝔑 |= (ϕ)[Γ].
+Fixpoint shift_vars n x :=
+  match x with
+  | Zero    => Zero
+  | One     => One
+  | Var i   => Var (n + i)
+  | Add x y => Add (shift_vars n x) (shift_vars n y)
+  end.
+
+Notation "# i" := (Var i) (at level 9, format "# i").
+Notation "x << n" := (shift_vars n x) (at level 10, format "x << n").
+
+Theorem eval_shift_vars x Γ n :
+  eval Γ (x<<n) = eval (skipn n Γ) x.
 Proof.
-Admitted.
+induction x; simpl. 1,2: easy.
+- revert Γ; induction n; simpl; intros.
+  easy. destruct Γ; simpl. now destruct i. apply IHn.
+- now rewrite IHx1, IHx2.
+Qed.
 
-End Embeddings.
+Lemma reduce_std_term j x n :
+  Σ ϕ, ∀Γ, Nat |= (Std_eq #j (x<<n))[Γ] <-> NatR |= (ϕ)[Γ].
+Proof.
+revert j n; induction x; intros.
+- now exists (R_zero j).
+- now exists (R_one j).
+- now exists (R_eq j (n + i)).
+- destruct (IHx1 0 (2 + n)) as [ϕ1 Hϕ1];
+  destruct (IHx2 1 (2 + n)) as [ϕ2 Hϕ2].
+  exists ∃[∃[R_add (2 + j) 0 1 ∧` ϕ1 ∧` ϕ2]].
+  simpl in *; split.
+  + intros H. exists (eval Γ (x2<<n)), (eval Γ (x1<<n)).
+    repeat split. easy.
+    * apply Hϕ1; simpl. now rewrite ?eval_shift_vars.
+    * apply Hϕ2; simpl. now rewrite ?eval_shift_vars.
+  + intros [n2 [n1 [H [H1 H2]]]].
+    apply Hϕ1 in H1; rewrite eval_shift_vars in H1;
+    apply Hϕ2 in H2; rewrite eval_shift_vars in H2; simpl in *.
+    rewrite ?eval_shift_vars; congruence.
+Qed.
+
+Lemma reduce_std_eq x y Γ :
+  Nat |= (Std_eq x y)[Γ] <-> 
+  Nat |= (∃[Std_eq #0 (x<<1) ∧` Std_eq #0 (y<<1)])[Γ].
+Proof.
+split; simpl.
+- intros H. exists (eval Γ x).
+  split; now rewrite eval_shift_vars.
+- intros [n [H1 H2]].
+  rewrite eval_shift_vars in H1;
+  rewrite eval_shift_vars in H2;
+  simpl in *; congruence.
+Qed.
+
+Lemma reduce_std_le x y Γ :
+  Nat |= (Std_le x y)[Γ] <-> 
+  Nat |= (∃[∃[Std_le #0 #1 ∧` Std_eq #0 (x<<2) ∧` Std_eq #1 (y<<2)]])[Γ].
+Proof.
+split; simpl.
+- intros H; exists (eval Γ y), (eval Γ x); repeat split.
+  easy. all: now rewrite eval_shift_vars.
+- intros [n2 [n1 [H [H1 H2]]]].
+  rewrite eval_shift_vars in H1;
+  rewrite eval_shift_vars in H2;
+  simpl in *; congruence.
+Qed.
+
+Lemma std_le_iff_r_le i j Γ :
+  Nat |= (Std_le #i #j)[Γ] <-> NatR |= (R_le i j)[Γ].
+Proof.
+easy.
+Qed.
+
+Theorem convert_std_atom_to_rformula (a : std_atom) :
+  Σ ϕ, ∀Γ, NatR |= (ϕ)[Γ] <-> Nat |= (a)[Γ].
+Proof.
+destruct a.
+- (* Equality relation. *)
+  destruct reduce_std_term with (j:=0)(x:=x)(n:=1) as [ϕx Hx];
+  destruct reduce_std_term with (j:=0)(x:=y)(n:=1) as [ϕy Hy].
+  eexists; symmetry; etransitivity. apply reduce_std_eq.
+  apply realizes_ex, realizes_and; easy.
+- (* Less or equal relation. *)
+  destruct reduce_std_term with (j:=0)(x:=x)(n:=2) as [ϕx Hx].
+  destruct reduce_std_term with (j:=1)(x:=y)(n:=2) as [ϕy Hy].
+  eexists; symmetry; etransitivity. apply reduce_std_le.
+  apply realizes_ex, realizes_ex, realizes_and.
+  apply std_le_iff_r_le. apply realizes_and; easy.
+Qed.
+
+Corollary convert_formula_to_rformula φ :
+  Σ ϕ, ∀Γ, NatR |= (ϕ)[Γ] <-> Nat |= (φ)[Γ].
+Proof.
+induction φ.
+- apply convert_std_atom_to_rformula.
+- destruct IHφ1 as [ϕ1 H1], IHφ2 as [ϕ2 H2].
+  exists (ϕ1 ∧` ϕ2); split.
+  all: split; [apply H1|apply H2]; apply H.
+- destruct IHφ as [ϕ H].
+  exists (¬`ϕ); split; apply contra, H.
+- destruct IHφ as [ϕ H].
+  exists ∃[ϕ]; split;
+  intros [x Hx]; exists x; apply H, Hx.
+Qed.
+
+End Embedding_of_formula_in_rformula.
