utilities.v
@@ -58,39 +58,7 @@ End Propositions.
 End Laws_of_logic.
 
 (******************************************************************************)
-(* II. Editing arbitrary infinite sequences.                                  *)
-(******************************************************************************)
-Section Editing_sequences.
-
-Variable X : Type.
-
-Definition set n (x : X) Γ i := if i =? n then x else Γ i.
-
-Variable Γ : nat -> X.
-Variable i j k : nat.
-Variable x y : X.
-
-Lemma set_override :
-  set i x (set i y Γ) k = set i x Γ k.
-Proof.
-unfold set; now destruct (k =? i).
-Qed.
-
-Lemma set_swap :
-  i ≠ j -> set i x (set j y Γ) k = set j y (set i x Γ) k.
-Proof.
-unfold set; destruct (k =? i) eqn:I, (k =? j) eqn:J; try easy.
-b_Prop; subst; easy.
-Qed.
-
-End Editing_sequences.
-
-Arguments set {_}.
-Notation "α ;; n ↦ x" := (set n x α)
-  (at level 25, left associativity, format "α ;; n ↦ x").
-
-(******************************************************************************)
-(* III. Various list utilities.                                               *)
+(* II. Various list utilities.                                               *)
 (******************************************************************************)
 Section Lemmas_about_lists.
 
